more cleanup

Imp/Aexp.lean
@@ -3,13 +3,15 @@ import Imp.Syntax
 
 import Mathlib.Init.Function
 
+namespace Aexp
+
 -- Operational semantics of aexp
-inductive Aexp.Nat: Aexp × State → Int → Prop
+inductive Nat: Aexp × State → Int → Prop
   | num₁:
     Nat (num n, _) n
 
   | loc₁:
-    Nat (loc x, s) (s↓x)
+    Nat (loc x, s) (s⇓x)
 
   | add₁ (h₁: Nat (a,s) n) (h₂: Nat (b,s) m):
     Nat (add a b, s) (n + m)
@@ -20,27 +22,27 @@ inductive Aexp.Nat: Aexp × State → Int → Prop
   | mul₁ (h₁: Nat (a,s) n) (h₂: Nat (b,s) m):
     Nat (mul a b, s) (n * m)
 
-infix:110 " ⟹ " => Aexp.Nat
+infix:110 " ⟹ " => Nat
 
 -- Denotational semantics of arithmetic expressions
-@[reducible] def Aexp.red (a: Aexp) (s: State): Int :=
+@[reducible] def red (a: Aexp) (s: State): Int :=
   match a with
   | num n => n
-  | loc x => s↓x
+  | loc x => s⇓x
   | add a b => red a s + red b s
   | sub a b => red a s - red b s
   | mul a b => red a s * red b s
 
-infix:110 "↓" => Aexp.red
+infix:110 "⇓" => red
 
 -- relational definition is equal to recursive
-theorem Aexp.red.from_Nat (h: as ⟹ n): red.uncurry as = n :=
+theorem red.from_Nat (h: as ⟹ n): red.uncurry as = n :=
   by induction h with
   | num₁ => rfl
   | loc₁ => rfl
   | _ _ _ ih₁ ih₂ => exact ih₁ ▸ ih₂ ▸ rfl
 
-theorem Aexp.Nat.from_red {a: Aexp} (h: a↓s = n): (a,s) ⟹ n :=
+theorem Nat.from_red {a: Aexp} (h: a⇓s = n): (a,s) ⟹ n :=
   by induction a generalizing n with
   | num _ => exact h ▸ num₁
   | loc _ => exact h ▸ loc₁
@@ -48,10 +50,10 @@ theorem Aexp.Nat.from_red {a: Aexp} (h: a↓s = n): (a,s) ⟹ n :=
   | sub _ _ l r => exact h ▸ sub₁ (l rfl) (r rfl)
   | mul _ _ l r => exact h ▸ mul₁ (l rfl) (r rfl)
 
-@[simp] theorem Aexp.Nat_iff_red: (a, s) ⟹ n ↔ a↓s = n := ⟨red.from_Nat, Nat.from_red⟩
-@[simp] theorem Aexp.Nat_iff_red': (a, s) ⟹ (a↓s) := Nat.from_red rfl
+@[simp] theorem Nat_iff_red: (a, s) ⟹ n ↔ a⇓s = n := ⟨red.from_Nat, Nat.from_red⟩
+@[simp] theorem Nat_iff_red': (a, s) ⟹ (a⇓s) := Nat.from_red rfl
 
-protected instance Aexp.Nat.equiv: Setoid Aexp where
+protected instance Nat.equiv: Setoid Aexp where
   r a b := ∀ s n, (a, s) ⟹ n = (b, s) ⟹ n
   iseqv := {
     refl := λ _ _ _ ↦ Eq.refl _
@@ -59,7 +61,7 @@ protected instance Aexp.Nat.equiv: Setoid Aexp where
     trans := λ h₁ h₂ x n ↦ (h₁ x n) ▸ (h₂ x n)
   }
 
-instance Aexp.red.equiv: Setoid Aexp where
+instance red.equiv: Setoid Aexp where
   r := (red · = red ·)
   iseqv := {
     refl := λ _ ↦ Eq.refl _
@@ -67,14 +69,16 @@ instance Aexp.red.equiv: Setoid Aexp where
     trans := (· ▸ ·)
   }
 
-protected theorem Aexp.Nat_eq_eq_red_eq: Aexp.Nat.equiv.r a b ↔ Aexp.red.equiv.r a b :=
+protected theorem Nat_eq_eq_red_eq: Nat.equiv.r a b ↔ red.equiv.r a b :=
   by
   constructor <;> intro h
   . simp [Setoid.r] at *
     apply funext
     intro s
-    specialize h s (b↓s)
+    specialize h s (b⇓s)
     simp at h
     exact h
   . simp [Setoid.r] at *
     simp [h]
+
+end Aexp
