Imp/Bexp.lean
@@ -1,7 +1,9 @@
 import Imp.Aexp
 
+namespace Bexp
+
 -- Operational semantics of Bexp
-inductive Bexp.Nat: Bexp × State → Bool → Prop
+inductive Nat: Bexp × State → Bool → Prop
   | tt₁:
     Nat (tt, _) true
 
@@ -9,10 +11,10 @@ inductive Bexp.Nat: Bexp × State → Bool → Prop
     Nat (ff, _) false
 
   | eq₁:
-    Nat (eq a b, s) (a↓s = b↓s)
+    Nat (eq a b, s) (a⇓s = b⇓s)
 
   | le₁:
-    Nat (le a b, s) (a↓s ≤ b↓s)
+    Nat (le a b, s) (a⇓s ≤ b⇓s)
 
   | not₁ {a: Bexp} (h: Nat (a,s) n):
     Nat (not a, s) (!n)
@@ -23,23 +25,23 @@ inductive Bexp.Nat: Bexp × State → Bool → Prop
   | or₁ {a b: Bexp} (h₁: Nat (a,s) n) (h₂: Nat (b,s) m):
     Nat (or a b, s) (n || m)
 
-infix:110 " ⟹ " => Bexp.Nat
+infix:110 " ⟹ " => Nat
 
 -- Denotational semantics of Bexp
-@[reducible, simp] def Bexp.red (b: Bexp) (s: State): Bool :=
+@[reducible, simp] def red (b: Bexp) (s: State): Bool :=
   match b with
   | tt      => true
   | ff      => false
   | not b   => !red b s
   | and a b => red a s && red b s
   | or a b  => red a s || red b s
-  | eq a b  => a↓s = b↓s
-  | le a b  => a↓s ≤ b↓s
+  | eq a b  => a⇓s = b⇓s
+  | le a b  => a⇓s ≤ b⇓s
 
-infix:110 "↓" => Bexp.red
+infix:110 "⇓" => red
 
 -- relational definition is equivalent to recursive
-theorem Bexp.Nat.from_red {b: Bexp} (h: b↓s = x): (b,s) ⟹ x :=
+theorem Nat.from_red {b: Bexp} (h: b⇓s = x): (b, s) ⟹ x :=
   by induction b generalizing x with
   | tt => exact h ▸ Nat.tt₁
   | ff => exact h ▸ Nat.ff₁
@@ -49,7 +51,7 @@ theorem Bexp.Nat.from_red {b: Bexp} (h: b↓s = x): (b,s) ⟹ x :=
   | and _ _ l r => exact h ▸ Nat.and₁ (l rfl) (r rfl)
   | or _ _  l r => exact h ▸ Nat.or₁  (l rfl) (r rfl)
 
-theorem Bexp.red.from_Nat {bs: Bexp × State} (h: bs ⟹ x): red.uncurry bs = x :=
+theorem red.from_Nat {bs: Bexp × State} (h: bs ⟹ x): red.uncurry bs = x :=
   by induction h with
   | tt₁ => rfl
   | ff₁ => rfl
@@ -58,11 +60,11 @@ theorem Bexp.red.from_Nat {bs: Bexp × State} (h: bs ⟹ x): red.uncurry bs = x 
   | not₁ _ ih => exact ih ▸ rfl
   | _ _ _ ih₁ ih₂ => exact ih₁ ▸ ih₂ ▸ rfl
 
-@[simp] theorem Bexp.Nat_eq_red {b: Bexp}: (b,s) ⟹ r ↔ b↓s = r := ⟨red.from_Nat, Nat.from_red⟩
+@[simp] theorem Nat_eq_red {b: Bexp}: (b,s) ⟹ r ↔ b⇓s = r := ⟨red.from_Nat, Nat.from_red⟩
 
-theorem Bexp.not_true_eq_false: (!b↓s) = (not b)↓s := by simp
+theorem not_true_eq_false: (!b⇓s) = (not b)⇓s := by simp
 
-protected instance Bexp.Nat.equiv: Setoid Bexp where
+protected instance Nat.equiv: Setoid Bexp where
   r a b := ∀ s n, (a, s) ⟹ n = (b, s) ⟹ n
   iseqv := {
     refl := λ _ _ _ ↦ Eq.refl _
@@ -70,7 +72,7 @@ protected instance Bexp.Nat.equiv: Setoid Bexp where
     trans := λ h₁ h₂ x n ↦ (h₁ x n) ▸ (h₂ x n)
   }
 
-instance Bexp.red.equiv: Setoid Bexp where
+instance red.equiv: Setoid Bexp where
   r := (red · = red ·)
   iseqv := {
     refl := λ _ ↦ Eq.refl _
@@ -78,14 +80,16 @@ instance Bexp.red.equiv: Setoid Bexp where
     trans := (· ▸ ·)
   }
 
-protected theorem Bexp.Nat_eq_eq_red_eq: Bexp.Nat.equiv.r a b ↔ Bexp.red.equiv.r a b :=
+protected theorem Nat_eq_eq_red_eq: Nat.equiv.r a b ↔ red.equiv.r a b :=
   by
   constructor <;> intro h
   . simp [Setoid.r] at *
     apply funext
     intro s
-    specialize h s (b↓s)
+    specialize h s (b⇓s)
     simp at h
     exact h
   . simp [Setoid.r] at *
     simp [h]
+
+end Bexp
