Imp/Denot.lean
@@ -5,64 +5,71 @@ import Mathlib.Order.CompleteLattice
 import Mathlib.Data.Set.Lattice
 import Mathlib.Order.FixedPoints
 
--- Set relation denotational semantics,
--- aka graph of partial function
-@[reducible]
-def SRel α β := Set (α × β)
+namespace SRel
 
-infixl:20 " →ˢ " => SRel
+/-!
+## Set relation `Set (α × β)`, aka graph of partial function, aka Lana Del Rey
+-/
 
-def SRel.id: α →ˢ α := {p | p.1 = p.2}
+notation:20 α " →ˢ " β => Set (α × β)
 
-@[simp] theorem SRel.mem_id {a b: α}:
+def id: α →ˢ α := {p | p.1 = p.2}
+
+@[simp] theorem mem_id {a b: α}:
   (a, b) ∈ @id α ↔ a = b := Iff.rfl
 
-def SRel.comp (f g: α →ˢ α): α →ˢ α :=
+def comp (f g: α →ˢ α): α →ˢ α :=
   {x | ∃z, (x.1, z) ∈ f ∧ (z, x.2) ∈ g}
 
 infixl:90 " ○ " => SRel.comp
 
-@[simp] theorem SRel.mem_comp {f g: α →ˢ α}:
+@[simp] theorem mem_comp {f g: α →ˢ α}:
   x ∈ f ○ g ↔ ∃z, (x.1, z) ∈ f ∧ (z, x.2) ∈ g := Iff.rfl
 
 @[reducible]
-def SRel.restrict (f: α →ˢ β) (s: Set α): α →ˢ β :=
+def restrict (s: Set α) (f: α →ˢ β): α →ˢ β :=
   {x ∈ f | x.1 ∈ s}
 
-theorem SRel.monotone_comp [PartialOrder α] {f g: α → (β →ˢ β)}
+theorem monotone_comp [PartialOrder α] {f g: α → (β →ˢ β)}
   (hf: Monotone f) (hg: Monotone g):
   Monotone λ x ↦ f x ○ g x :=
   λ _ _ h _ ⟨z, h₁, h₂⟩ => ⟨z, hf h h₁, hg h h₂⟩
 
-theorem SRel.monotone_restrict [PartialOrder α] {f : α → (β →ˢ β)} {s: Set β}
+theorem monotone_restrict [PartialOrder α] {f : α → (β →ˢ β)} {s: Set β}
   (hf: Monotone f):
-  Monotone λ x ↦ restrict (f x) s :=
+  Monotone (restrict s $ f ·) :=
   λ _ _ h _ ⟨z, h₁⟩ ↦ ⟨hf h z, h₁⟩
 
-def Com.Γ (b: Bexp) (f: State →ˢ State): (State →ˢ State) →o (State →ˢ State) := {
-  toFun := λ g ↦ ((f ○ g).restrict {s | b↓s = true})
-                    ∪ (SRel.id.restrict {s | b↓s = false})
+end SRel
+
+namespace Com
+
+def Γ (b: Bexp) (f: State →ˢ State): (State →ˢ State) →o (State →ˢ State) := {
+  toFun := λ g ↦ (SRel.restrict {s | b⇓s = true} (f ○ g))
+                    ∪ (SRel.restrict {s | b⇓s = false} SRel.id)
   monotone' :=
     Monotone.union
     (SRel.monotone_restrict (SRel.monotone_comp monotone_const monotone_id))
     (SRel.monotone_restrict monotone_const)
 }
 
-def Com.denot: Com → (State →ˢ State)
+def denot: Com → (State →ˢ State)
   | skip       => SRel.id
-  | ass x a    => {s | s.2 = s.1⟦x↦a↓s.1⟧}
+  | ass x a    => {s | s.2 = s.1⟦x↦a⇓s.1⟧}
   | c;;d       => c.denot ○ d.denot
-  | cond b c d => (c.denot.restrict {s | b↓s = true})
-                    ∪ (d.denot.restrict {s | b↓s = false})
+  | cond b c d => (SRel.restrict {s | b⇓s = true} c.denot)
+                    ∪ (SRel.restrict {s | b⇓s = false} d.denot)
   | wle b c    => OrderHom.lfp (Γ b c.denot)
 
-notation (priority := high) "⟦" c "⟧" => Com.denot c
+notation (priority := high) "⟦" c "⟧" => denot c
 
 #simp (⟦⟧, ⟦"x"↦5⟧⟦"x"↦1⟧) ∈ ⟦⦃x = 5; if x == 1 {skip} else {x = 1}⦄⟧
 #simp (⟦⟧, ⟦"x"↦5⟧) ∈ ⟦⦃x = 5; while x == 1 {x = 1}⦄⟧
 
+namespace denot
+
 @[simp]
-instance Com.denot.equiv: Setoid Com where
+instance equiv: Setoid Com where
   r := (⟦·⟧ = ⟦·⟧)
   iseqv := {
     refl := λ _ ↦ Eq.refl _
@@ -70,33 +77,36 @@ instance Com.denot.equiv: Setoid Com where
     trans := (· ▸ ·)
   }
 
-theorem Com.denot.cat_congr (hc: c₁ ≈ c₂) (hd: d₁ ≈ d₂):
+theorem cat_congr (hc: c₁ ≈ c₂) (hd: d₁ ≈ d₂):
   (c₁;;d₁) ≈ (c₂;;d₂) :=
   by
     simp [HasEquiv.Equiv, denot]
     exact hc ▸ hd ▸ rfl
 
-theorem Com.denot.cond_congr (hc: c₁ ≈ c₂) (hd: d₁ ≈ d₂):
+theorem cond_congr (hc: c₁ ≈ c₂) (hd: d₁ ≈ d₂):
   (cond b c₁ d₁) ≈ (cond b c₂ d₂) :=
   by
     simp [HasEquiv.Equiv, denot]
     exact hc ▸ hd ▸ rfl
 
-theorem Com.denot.wle_congr (hc: c₁ ≈ c₂):
+theorem wle_congr (hc: c₁ ≈ c₂):
   (wle b c₁) ≈ (wle b c₂) :=
   by
     simp [HasEquiv.Equiv, denot]
     exact hc ▸ rfl
 
-theorem Com.denot.cat_skipl:
+theorem skipl:
   (skip;;c) ≈ c :=
   by simp [HasEquiv.Equiv, denot, SRel.comp]
 
-theorem Com.denot.cat_skipr:
+theorem skipr:
   (c;;skip) ≈ c :=
   by simp [HasEquiv.Equiv, denot, SRel.comp]
 
-theorem Com.denot.wle_unfold:
+theorem wle_unfold:
   wle b c ≈ cond b (c;;wle b c) skip := by
   simp [HasEquiv.Equiv]
   exact Eq.symm (OrderHom.map_lfp (Γ b ⟦c⟧))
+
+end denot
+end Com
