Imp/Natural.lean
@@ -1,43 +1,47 @@
 import Imp.Bexp
 
-inductive Com.Nat: Com × State → State → Prop
+namespace Com
+
+inductive Nat: Com × State → State → Prop
   | skip₁:
     Nat (skip, s) s
 
   | ass₁:
-    Nat (ass x a, s) (s⟦x↦a↓s⟧)
+    Nat (ass x a, s) (s⟦x↦a⇓s⟧)
 
   | cat₁ t
     (hc: Nat (c, s) t) (hd: Nat (d, t) u):
     Nat (c;;d, s) u
 
   | cond₁ {b: Bexp}
-    (hb: b↓s = true) (hc: Nat (c, s) t):
+    (hb: b⇓s = true) (hc: Nat (c, s) t):
     Nat (cond b c d, s) t
 
   | cond₂ {b: Bexp}
-    (hb: b↓s = false) (hd: Nat (d, s) t):
+    (hb: b⇓s = false) (hd: Nat (d, s) t):
     Nat (cond b c d, s) t
 
   | wle₁ {b: Bexp} u
-    (hb: b↓s = true) (hc: Nat (c, s) u) (hw: Nat (wle b c, u) t):
+    (hb: b⇓s = true) (hc: Nat (c, s) u) (hw: Nat (wle b c, u) t):
     Nat (wle b c, s) t
 
   | wle₂ {b: Bexp}
-    (hb: b↓s = false):
+    (hb: b⇓s = false):
     Nat (wle b c, s) s
 
-infix:110 " ⟹ " => Com.Nat
+infix:110 " ⟹ " => Nat
 
-theorem Com.Nat.demo₁: (⦃x = 5⦄, ⟦⟧) ⟹ ⟦"x"↦5⟧ := ass₁
+namespace Nat
 
-theorem Com.Nat.demo₂:
+theorem demo₁: (⦃x = 5⦄, ⟦⟧) ⟹ ⟦"x"↦5⟧ := ass₁
+
+theorem demo₂:
   (⦃x = 2; if x <= 1 {y = 3} else {z = 4}⦄, ⟦⟧) ⟹
   (⟦"x"↦2⟧⟦"z"↦4⟧) := cat₁ _ ass₁ (cond₂ rfl ass₁)
 
-theorem Com.Nat.skip_same: (skip, s) ⟹ s₁ ↔ s = s₁ := ⟨(by cases .; rfl), (· ▸ skip₁)⟩
+theorem skip_same: (skip, s) ⟹ s₁ ↔ s = s₁ := ⟨(by cases .; rfl), (· ▸ skip₁)⟩
 
-instance Com.Nat.equiv: Setoid Com where
+instance equiv: Setoid Com where
   r c d := ∀ s t, (c, s) ⟹ t = (d, s) ⟹ t
   iseqv := {
     refl := λ _ _ _ ↦ Eq.refl _
@@ -45,7 +49,7 @@ instance Com.Nat.equiv: Setoid Com where
     trans := λ h₁ h₂ x n ↦ (h₁ x n) ▸ (h₂ x n)
   }
 
-theorem Com.Nat.skipl: (skip;;c) ≈ c := by
+theorem skipl: (skip;;c) ≈ c := by
   intro _ _
   apply propext
   constructor
@@ -53,7 +57,7 @@ theorem Com.Nat.skipl: (skip;;c) ≈ c := by
     exact skip_same.mp hc ▸ hd
   . exact (cat₁ _ skip₁ ·)
 
-theorem Com.Nat.skipr: (c;;skip) ≈ c := by
+theorem skipr: (c;;skip) ≈ c := by
   intro _ _
   apply propext
   constructor
@@ -61,26 +65,26 @@ theorem Com.Nat.skipr: (c;;skip) ≈ c := by
     exact skip_same.mp hd ▸ hc
   . exact (cat₁ _ · skip₁)
 
-theorem Com.Nat.cond_tt (h: b ≈ Bexp.tt): cond b c d ≈ c := by
+theorem cond_tt (h: b ≈ Bexp.tt): cond b c d ≈ c := by
   intro _ _; apply propext; constructor <;> intro h₁
   . cases h₁ with
     | cond₁ => assumption
     | cond₂ hb => rw [h] at hb; contradiction
-  . exact Nat.cond₁ (h ▸ rfl) h₁
+  . exact cond₁ (h ▸ rfl) h₁
 
-theorem Com.Nat.cond_ff (h: b ≈ Bexp.ff): cond b c d ≈ d := by
+theorem cond_ff (h: b ≈ Bexp.ff): cond b c d ≈ d := by
   intro _ _; apply propext; constructor <;> intro h₁
   . cases h₁ with
     | cond₂ => assumption
     | cond₁ hb => rw [h] at hb; contradiction
-  . exact Nat.cond₂ (h ▸ rfl) h₁
+  . exact cond₂ (h ▸ rfl) h₁
 
-theorem Com.Nat.wle_unfold:
+theorem wle_unfold:
   wle b c ≈ cond b (c;;wle b c) skip := by
   intro s t
   apply propext
   constructor <;> intro h
-  . cases hb: b↓s
+  . cases hb: b⇓s
     . apply cond₂ hb
       cases h
       . rw [hb] at *; contradiction
@@ -89,7 +93,7 @@ theorem Com.Nat.wle_unfold:
       cases h
       . constructor <;> assumption
       . rw [hb] at *; contradiction
-  . cases hb: b↓s
+  . cases hb: b⇓s
     . cases h
       . rw [hb] at *; contradiction
       . rename_i hd; cases hd; apply wle₂; assumption
@@ -97,8 +101,8 @@ theorem Com.Nat.wle_unfold:
       . rename_i hc; cases hc; constructor <;> assumption
       . rw [hb] at *; contradiction
 
-theorem Com.Nat.cond_ext: (cond b c d, s) ⟹ t ↔ bif b↓s then (c, s) ⟹ t else (d, s) ⟹ t := by
-  constructor <;> intro h <;> cases hb: b↓s <;> simp at *
+theorem cond_ext: (cond b c d, s) ⟹ t ↔ bif b⇓s then (c, s) ⟹ t else (d, s) ⟹ t := by
+  constructor <;> intro h <;> cases hb: b⇓s <;> simp at *
   . cases h
     simp [hb] at *
     assumption
@@ -110,16 +114,16 @@ theorem Com.Nat.cond_ext: (cond b c d, s) ⟹ t ↔ bif b↓s then (c, s) ⟹ t 
   . rw [hb] at h
     exact cond₁ hb h
 
-theorem Com.Nat.cond_ext': (cond b c d, s) ⟹ t ↔ (bif b↓s then c else d, s) ⟹ t := by
-  rw [cond_ext]; cases b↓s <;> simp
+theorem cond_ext': (cond b c d, s) ⟹ t ↔ (bif b⇓s then c else d, s) ⟹ t := by
+  rw [cond_ext]; cases b⇓s <;> simp
 
-theorem Com.Nat.cond_ext'': (cond b c d, s) ⟹ t ↔ (bif b↓s then (c, s) else (d, s)) ⟹ t := by
-  rw [cond_ext]; cases b↓s <;> simp
+theorem cond_ext'': (cond b c d, s) ⟹ t ↔ (bif b⇓s then (c, s) else (d, s)) ⟹ t := by
+  rw [cond_ext]; cases b⇓s <;> simp
 
-theorem Com.Nat.wle_iff:
+theorem wle_iff:
   (wle b c, s) ⟹ u ↔
-  (∃t, b↓s ∧ (c, s) ⟹ t ∧ (wle b c, t) ⟹ u)
-  ∨ (¬ b↓s ∧ u = s) :=
+  (∃t, b⇓s ∧ (c, s) ⟹ t ∧ (wle b c, t) ⟹ u)
+  ∨ (¬ b⇓s ∧ u = s) :=
   by
     apply Iff.intro
     . intro h
@@ -149,7 +153,7 @@ theorem Com.Nat.wle_iff:
           apply wle₂
           simp [*]
 
-theorem Com.Nat.wle_tt (heqb: b ≈ Bexp.tt):
+theorem wle_tt (heqb: b ≈ Bexp.tt):
   ¬((wle b c, s) ⟹ t) := by
   intro h₁
   generalize h₂: (wle b c, s) = ww at h₁
@@ -158,7 +162,7 @@ theorem Com.Nat.wle_tt (heqb: b ≈ Bexp.tt):
   | wle₂ hb => cases h₂; rw [heqb] at hb; contradiction
   | _ => cases h₂
 
-theorem Com.Nat.determ {cs: Com × State} (h₁: cs ⟹ t) (h₂: cs ⟹ u): t = u :=
+theorem determ {cs: Com × State} (h₁: cs ⟹ t) (h₂: cs ⟹ u): t = u :=
   by induction h₁ generalizing u with
   | cat₁ _ _ _ ih₁ ih₂ => cases h₂ with
     | cat₁ _ hc hd => exact ih₂ (ih₁ hc ▸ hd)
@@ -180,3 +184,6 @@ theorem Com.Nat.determ {cs: Com × State} (h₁: cs ⟹ t) (h₂: cs ⟹ u): t =
     | wle₂ => rfl
 
   | _ => cases h₂; rfl
+
+end Nat
+end Com
