Imp/Structural.lean
@@ -2,9 +2,11 @@ import Imp.Bexp
 
 import Mathlib.Logic.Relation
 
-inductive Com.Step: Com × State → Com × State → Prop
+namespace Com
+
+inductive Step: Com × State → Com × State → Prop
   | ass₁:
-    Step (ass x a, s) (skip, s⟦x↦a↓s⟧)
+    Step (ass x a, s) (skip, s⟦x↦a⇓s⟧)
 
   | cat₁:
     Step (skip;;c, s) (c, s)
@@ -13,18 +15,20 @@ inductive Com.Step: Com × State → Com × State → Prop
     Step (c;;d, s) (e;;d, t)
 
   | cond₁:
-    Step (cond b c d, s) (bif b↓s then (c, s) else (d, s))
+    Step (cond b c d, s) (bif b⇓s then (c, s) else (d, s))
 
   | wle₁:
     Step (wle b c, s) (cond b (c;;wle b c) skip, s)
 
-infix:110 " ⇒ " => Com.Step
+infix:110 " ⇒ " => Step
 
-theorem Com.Step.demo₁:
+namespace Step
+
+theorem Step.demo₁:
   (⦃x = 2; while 0 <= x {x = x - 1}⦄, ⟦⟧) ⇒
       (⦃skip; while 0 <= x {x = x - 1}⦄, ⟦"x"↦2⟧) := cat₂ ass₁
 
-@[simp] theorem Com.Step.cat_iff:
+@[simp] theorem cat_iff:
   (c₁;;c₂, s) ⇒ et ↔
   (∃e t, (c₁, s) ⇒ (e, t) ∧ et = (e;;c₂, t))
   ∨ (c₁ = skip ∧ et = (c₂, s)) :=
@@ -42,51 +46,57 @@ theorem Com.Step.demo₁:
       cases h with | intro h₁ h₂ =>
         exact h₁ ▸ h₂ ▸ Step.cat₁
 
-@[simp] lemma Com.Step.cond_iff:
+@[simp] lemma cond_iff:
   (cond b c d, s) ⇒ ss ↔
-  (b↓s ∧ ss = (c, s)) ∨ (b↓s = false ∧ ss = (d, s)) :=
+  (b⇓s ∧ ss = (c, s)) ∨ (b⇓s = false ∧ ss = (d, s)) :=
   by
   constructor <;> intro h
-  . cases hb: b↓s <;> cases h
+  . cases hb: b⇓s <;> cases h
     . exact Or.inr ⟨rfl, hb ▸ rfl⟩
     . exact Or.inl ⟨rfl, hb ▸ rfl⟩
-  . have hss: ss = bif b↓s then (c,s) else (d,s) := by
-      cases hb: b↓s <;> rw [hb] at h <;> simp at * <;> assumption
+  . have hss: ss = bif b⇓s then (c,s) else (d,s) := by
+      cases hb: b⇓s <;> rw [hb] at h <;> simp at * <;> assumption
     exact hss ▸ cond₁
 
-@[simp] lemma Com.Step.cond_false {b: Bexp} (hb: b↓s = false):
+@[simp] lemma cond_false {b: Bexp} (hb: b⇓s = false):
   (cond b c d, s) ⇒ ss ↔ (ss = (d, s)) :=
   by rw [cond_iff, hb]; simp
 
+end Step
+
 open Relation
 
-alias Com.Star        := ReflTransGen
-alias Com.Star.head   := ReflTransGen.head
-alias Com.Star.trans  := ReflTransGen.trans
-alias Com.Star.refl   := ReflTransGen.refl
-alias Com.Star.single := ReflTransGen.single
-alias Com.Star.lift   := ReflTransGen.lift
-alias Com.Star.head_induction_on := ReflTransGen.head_induction_on
+namespace Star
 
-infix:110 " ⇒* " => Com.Star Com.Step
+alias head   := ReflTransGen.head
+alias trans  := ReflTransGen.trans
+alias refl   := ReflTransGen.refl
+alias single := ReflTransGen.single
+alias lift   := ReflTransGen.lift
+alias head_induction_on := ReflTransGen.head_induction_on
 
-theorem Com.Star.demo₂:
+infix:110 " ⇒* " => ReflTransGen Step
+
+theorem demo₂:
   (⦃x = 2; while 0 <= x {x = x - 1}⦄, ⟦⟧) ⇒*
       (⦃while 0 <= x {x = x - 1}⦄, (⟦"x"↦2⟧)) :=
   head (Step.cat₂ Step.ass₁) (head Step.cat₁ Star.refl)
 
-theorem Com.Star.cat_skip_cat
+theorem cat_skip_cat
   (h: (c, s) ⇒* (skip, t)):
   (c;;d, s) ⇒* (skip;;d, t) :=
   lift (λ (x: Com × State) ↦ (x.1;;d, x.2)) (λ _ _ h => Step.cat₂ h) h
 
-theorem Com.Star.cat
+theorem cat
   (h₁: (c₁, s) ⇒* (skip, s₁))
   (h₂: (c₂, s₁) ⇒* (skip, s₂)):
   (c₁;;c₂, s) ⇒* (skip, s₂) :=
   trans (cat_skip_cat h₁) (trans (single Step.cat₁) h₂)
 
-theorem Com.Star.cat_no_influence
+theorem cat_no_influence
   (h: (c₁, s) ⇒* (skip, s₁)):
   (c₁;;c₂, s) ⇒* (c₂, s₁) :=
   trans (cat_skip_cat h) (single Step.cat₁)
+
+end Star
+end Com
